theories/case_studies/dle/deep_locality_concrete.v
@@ -107,7 +107,7 @@ Proof.
     dle_trusted_stack_b dle_trusted_stack_e
     _ _ _ _
     (replicate 100 (WInt 0)) _ eq_refl
-    dle_stack_b dle_stack_e (replicate 100 (WInt 0)) _ _ _ _ _ _ _).
+    dle_stack_b dle_stack_e (replicate 100 (WInt 0)) _ _ _ _ _ _ _ _).
   - vm_compute; solve_addr.
   - vm_compute; solve_addr.
   - vm_compute; solve_addr.
@@ -124,6 +124,9 @@ Proof.
     unfold finz.le_lt in Hx, Hx'; cbn in Hx, Hx'; lia.
   - reflexivity.
   - vm_compute; reflexivity.
+  - unfold disjoint_from_heap, disjoint, set_disjoint_instance.
+    intros x Hx Hx'. rewrite !elem_of_finz_seq_between in Hx, Hx'.
+    unfold finz.le_lt in Hx, Hx'; cbn in Hx, Hx'; lia.
   - unfold disjoint_from_shadow, disjoint, set_disjoint_instance.
     intros x Hx Hx'. rewrite !elem_of_finz_seq_between in Hx, Hx'.
     unfold finz.le_lt in Hx, Hx'; cbn in Hx, Hx'; lia.
