theories/case_studies/heap_temporal_safety/heap_temporal_safety_concrete.v
@@ -126,7 +126,7 @@ Proof.
     hts_switcher_b hts_switcher_e hts_switcher_call hts_switcher_return
     hts_switcher_otype hts_trusted_stack_b hts_trusted_stack_e
     _ _ _ _ (replicate 100 (WInt 0)) _ eq_refl
-    hts_stack_b hts_stack_e (replicate 100 (WInt 0)) _ _ _ _ _ _ _).
+    hts_stack_b hts_stack_e (replicate 100 (WInt 0)) _ _ _ _ _ _ _ _).
   all: hts_compute_layout.
 Defined.
 
