theories/case_studies/lse_downward/lse_adequacy.v
@@ -58,7 +58,8 @@ Proof.
   pose proof (trusted_stack_disjoint_from_shadow switcher_cmpt).
   pose proof (switcher_base_not_shadow switcher_cmpt).
   pose proof (compartment_layout.switcher_base_not_heap switcher_cmpt).
-  refine (mkSwitcherLayoutWf _ _ _ _ _ _ _ _); cbn in *; auto.
+  pose proof (compartment_layout.switcher_disjoint_from_heap switcher_cmpt).
+  refine (mkSwitcherLayoutWf _ _ _ _ _ _ _ _ _); cbn in *; auto.
 Defined.
 
 Local Instance memory_layout_assertLayout `{memory_layout} : assertLayout.
