theories/logrel/monotone.v
@@ -664,6 +664,16 @@ Section monotone.
     by rewrite /heap_cap_valid /heap_cap_live Hb.
   Qed.
 
+  Lemma interp_monotone_cap_disjoint W W' C t p g b e a :
+    disjoint_from_heap b e ->
+    related_sts_pub_world W W' ->
+    interp W C (WCap t p g b e a) -∗ interp W' C (WCap t p g b e a).
+  Proof.
+    intros Hdisj Hrelated.
+    iApply interp_monotone_cap_valid; last done.
+    intros _. by apply heap_cap_valid_disjoint.
+  Qed.
+
   Lemma interp_monotone_nl_cap_nonheap W W' C t p g b e a :
     is_heap_address b = false -> disjoint_from_heap b e ->
     related_sts_priv_world W W' -> isLocalWord (WCap t p g b e a) = false ->
@@ -672,6 +682,17 @@ Section monotone.
     intros Hb Hdisj Hrelated Hnl.
     iApply interp_monotone_nl_cap_valid; try done.
     by rewrite /heap_cap_valid /heap_cap_live Hb.
+  Qed.
+
+  Lemma interp_monotone_nl_cap_disjoint W W' C t p g b e a :
+    disjoint_from_heap b e ->
+    related_sts_priv_world W W' ->
+    isLocalWord (WCap t p g b e a) = false ->
+    interp W C (WCap t p g b e a) -∗ interp W' C (WCap t p g b e a).
+  Proof.
+    intros Hdisj Hrelated Hnl.
+    iApply interp_monotone_nl_cap_valid; try done.
+    intros _. by apply heap_cap_valid_disjoint.
   Qed.
 
 Lemma interp_monotone_continuation
@@ -688,7 +709,7 @@ Proof.
   - iFrame.
   - iDestruct "Hcallee" as "[%Hheap Hcallee]".
     iSplit; first done.
-    iApply (interp_monotone_cap_nonheap with "Hcallee"); naive_solver.
+    iApply (interp_monotone_cap_disjoint with "Hcallee"); naive_solver.
   - destruct (is_untrusted_caller_frm a); first done.
     iIntros (W'' Hrel'). iApply "Hrestore". iPureIntro.
     eapply related_sts_pub_trans_world; eauto.
