theories/switcher/switcher.v
@@ -226,7 +226,8 @@ Section Switcher.
         disjoint_from_shadow b_trusted_stack e_trusted_stack;
 
         switcher_base_not_shadow : is_shadow_address b_switcher = false;
-        switcher_base_not_heap : is_heap_address b_switcher = false
+        switcher_base_not_heap : is_heap_address b_switcher = false;
+        switcher_disjoint_from_heap : disjoint_from_heap b_switcher e_switcher
       }.
 
   Lemma switcher_call_sentry_not_heap
